abbreviations

src/examples/GPU.MatMul.fst
@@ -4,14 +4,9 @@ module GPU.MatMul
 #push-options "--fuel 1 --ifuel 1"
 
 open GPU
-open FStar.Mul
-open Pulse
-open Pulse.Lib.Array
-open Pulse.Lib.BigStar
 
 module A    = Pulse.Lib.Array
 module SZ   = FStar.SizeT
-module U64  = FStar.UInt64
 module Defs = GPU.MatMul.Defs
 
 let matmul_single = Defs.matmul_single Defs.rows Defs.shared Defs.columns
@@ -20,9 +15,9 @@ let matmul = Defs.matmul Defs.rows Defs.shared Defs.columns
 ghost
 fn setup
   (size: SZ.t { size == SZ.(Defs.rows *^ Defs.columns) })
-  (ga1 : gpu_array U64.t (Defs.rows * Defs.shared)) (ga2 : gpu_array U64.t (Defs.shared * Defs.columns)) (gr : gpu_array U64.t size)
-  (v1: erased (Seq.Base.seq U64.t) { Seq.Base.length v1 == Defs.rows * Defs.shared })
-  (v2: erased (Seq.Base.seq U64.t) { Seq.Base.length v2 == Defs.shared * Defs.columns })
+  (ga1 : gpu_array u64 (Defs.rows * Defs.shared)) (ga2 : gpu_array u64 (Defs.shared * Defs.columns)) (gr : gpu_array u64 size)
+  (v1: erased (Seq.Base.seq u64) { Seq.Base.length v1 == Defs.rows * Defs.shared })
+  (v2: erased (Seq.Base.seq u64) { Seq.Base.length v2 == Defs.shared * Defs.columns })
   requires gpu_pts_to_array gr 's ** gpu_pts_to_array ga1 v1 ** gpu_pts_to_array ga2 v2
   ensures  bigstar 0 size (fun i ->
              Defs.kpre Defs.rows Defs.shared Defs.columns ga1 ga2 gr #v1 #v2 (hide (SZ.v size)) i)
@@ -49,30 +44,30 @@ fn setup
   gpu_array_slice_1 #4 #_ gr #f #v;
   bigstar_zip #3 #4 #5 0 size _ _;
   bigstar_map #5 #0 #0 #size #_ #_
-    (fun i -> Defs.fold_pre Defs.rows Defs.shared Defs.columns ga1 ga2 gr #v1 #v2 #(Seq.Base.cons #U64.t _ (Seq.Base.empty #U64.t)) size i);
+    (fun i -> Defs.fold_pre Defs.rows Defs.shared Defs.columns ga1 ga2 gr #v1 #v2 #(Seq.Base.cons #u64 _ (Seq.Base.empty #u64)) size i);
 
   bigstar_eta();
 }
 
 fn main
-  (a1 a2: array U64.t)
-  (v1: erased (Seq.Base.seq U64.t) { Seq.Base.length v1 == Defs.rows * Defs.shared })
-  (v2: erased (Seq.Base.seq U64.t) { Seq.Base.length v2 == Defs.shared * Defs.columns })
+  (a1 a2: array u64)
+  (v1: erased (Seq.Base.seq u64) { Seq.Base.length v1 == Defs.rows * Defs.shared })
+  (v2: erased (Seq.Base.seq u64) { Seq.Base.length v2 == Defs.shared * Defs.columns })
   requires cpu ** A.pts_to a1 v1 ** A.pts_to a2 v2
-  returns  ar: array U64.t
+  returns  ar: array u64
   ensures  cpu ** A.pts_to a1 v1 ** A.pts_to a2 v2 ** A.pts_to ar (matmul v1 v2)
 {
   open FStar.SizeT;
   let size = Defs.rows *^ Defs.columns;
-  let ar = Pulse.Lib.Array.alloc #U64.t 0UL size;
+  let ar = Pulse.Lib.Array.alloc #u64 0UL size;
 
-  let ga1 = gpu_array_alloc #U64.t (Defs.rows *^ Defs.shared);
-  let ga2 = gpu_array_alloc #U64.t (Defs.shared *^ Defs.columns);
+  let ga1 = gpu_array_alloc #u64 (Defs.rows *^ Defs.shared);
+  let ga2 = gpu_array_alloc #u64 (Defs.shared *^ Defs.columns);
 
   GPU.Array.gpu_memcpy_host_to_device a1 ga1 (Defs.rows *^ Defs.shared);
   GPU.Array.gpu_memcpy_host_to_device a2 ga2 (Defs.shared *^ Defs.columns);
   
-  let gr = gpu_array_alloc #U64.t size;
+  let gr = gpu_array_alloc #u64 size;
 
   setup size ga1 ga2 gr v1 v2;
 
@@ -110,14 +105,14 @@ fn main
 
   bigstar_rw_congr 0 size 
         (fun (i: nat{b2t (0 <= i) /\ b2t (i < size)}) ->
-          gpu_pts_to_array_slice #U64.t
+          gpu_pts_to_array_slice #u64
             #(Defs.rows * Defs.columns)
             gr
             #1.0R
             i
             (i + 1)
-            (Defs.singleton #U64.t
-                (reveal #U64.t
+            (Defs.singleton #u64
+                (reveal #u64
                     (hide (Defs.matmul_single Defs.rows
                         Defs.shared
                         Defs.columns
@@ -126,13 +121,13 @@ fn main
                         (hide #nat (i / Defs.columns))
                         (hide #nat (i % Defs.columns))
                         Defs.shared)))))
-        (fun i -> gpu_pts_to_array_slice #U64.t #size gr #1.0R i
+        (fun i -> gpu_pts_to_array_slice #u64 #size gr #1.0R i
             (i + 1)
-            (Defs.singleton #U64.t
-                (reveal #U64.t
-                    (hide (Seq.Base.index #U64.t
-                      (reveal #(Seq.Base.seq U64.t)
-                          (hide #(Seq.Base.seq U64.t) (Defs.matmul Defs.rows Defs.shared Defs.columns v1 v2)))
+            (Defs.singleton #u64
+                (reveal #u64
+                    (hide (Seq.Base.index #u64
+                      (reveal #(Seq.Base.seq u64)
+                          (hide #(Seq.Base.seq u64) (Defs.matmul Defs.rows Defs.shared Defs.columns v1 v2)))
                       i)))))
         (fun i -> Defs.lemma_matmul_index Defs.rows Defs.shared Defs.columns v1 v2 i);
 
