src/examples/matmul-opt/GPU.MatMulOpt.Barrier.fsti
@@ -2,33 +2,30 @@ module GPU.MatMulOpt.Barrier
 
 #lang-pulse
 
-open FStar.Mul
-open Pulse.Lib.Pervasives
-open Pulse.Lib.BigStar
 open GPU
+open GPU.Barrier.RPM
 module Pure = GPU.MatMulOpt.Pure
 module SZ = FStar.SizeT
-module U64 = FStar.UInt64
 
 #push-options "--admit_smt_queries true"
 let barrier_mm_share
     (n: nat)
-    (s1 s2: Seq.Base.seq (Seq.Base.seq U64.t))
-    (ar: gpu_array U64.t (2 * n))
-    (it: nat { it < Seq.Base.length s1 /\ it < Seq.Base.length s2 })
+    (s1 s2: seq (seq u64))
+    (ar: gpu_array u64 (2 * n))
+    (it: nat { it < Seq.length s1 /\ it < Seq.length s2 })
     (from: nat { 0 <= from /\ from < n })
     (to: nat { 0 <= to /\ to < n })
     : slprop
 =
   gpu_pts_to_array_slice ar #(1.0R /. Real.of_int n)
-    from (from + 1) (Pure.singleton (Seq.Base.index (Seq.Base.index s1 it) from)) **
+    from (from + 1) (Pure.singleton (Seq.index (Seq.index s1 it) from)) **
   gpu_pts_to_array_slice ar #(1.0R /. Real.of_int n)
-    (from + n) (from + n + 1) (Pure.singleton (Seq.Base.index (Seq.Base.index s2 it) from))
+    (from + n) (from + n + 1) (Pure.singleton (Seq.index (Seq.index s2 it) from))
 #pop-options
 
 let barrier_mm_gather
     (n: nat)
-    (ar: gpu_array U64.t (2 * n))
+    (ar: gpu_array u64 (2 * n))
     (it: nat)
     (from: nat { 0 <= from /\ from < n })
     (to: nat { 0 <= to /\ to < n })
@@ -37,35 +34,35 @@ let barrier_mm_gather
 
 let barrier_mm
     (n: nat)
-    (s1 s2: Seq.Base.seq (Seq.Base.seq U64.t)) //  { Seq.Base.length i == n }))
-    (ar: gpu_array U64.t (2 * n))
+    (s1 s2: seq (seq u64)) //  { Seq.length i == n }))
+    (ar: gpu_array u64 (2 * n))
     (it: nat)
     (from: nat { 0 <= from /\ from < n })
     (to: nat { 0 <= to /\ to < n })
     : slprop
 =
-  if (it / 2 < Seq.Base.length s1 && it / 2 < Seq.Base.length s2)
+  if (it / 2 < Seq.length s1 && it / 2 < Seq.length s2)
   then (cond (it % 2 = 0) (barrier_mm_share n s1 s2 ar (it / 2) from to) (barrier_mm_gather n ar (it / 2) from to))
   else emp
 
-let shared_pre (nthr : SZ.t { 0 < nthr /\ nthr <= max_threads })
-    (s1 s2: Seq.Base.seq (Seq.Base.seq U64.t))
-    (it: nat) (ar: gpu_array U64.t SZ.(2sz *^ nthr)) (i: nat { 0 <= i /\ i < nthr })
+let shared_pre (nthr : sz { 0 < nthr /\ nthr <= max_threads })
+    (s1 s2: seq (seq u64))
+    (it: nat) (ar: gpu_array u64 SZ.(2sz *^ nthr)) (i: nat { 0 <= i /\ i < nthr })
 : slprop
 = gpu_pts_to_array1 ar i **
   gpu_pts_to_array1 ar (i + nthr) ** mbarrier_tok nthr (barrier_mm nthr s1 s2 ar) it i
 
 ghost
 fn block_setup_ghost
-  (nblk : SZ.t { 0 < reveal nblk /\ reveal nblk <= max_blocks })
-  (nthr : SZ.t { 0 < nthr /\ nthr <= max_threads })
-  (smem_sz : SZ.t { smem_sz == SZ.(2sz *^ nthr) })
-  (ar: gpu_array U64.t smem_sz)
-  (bid: SZ.t { 0 <= bid /\ SZ.v bid < SZ.v nblk })
-  requires block_setup nthr ** (exists* v. gpu_pts_to_array #U64.t #smem_sz ar #1.0R v)
-  ensures block_setup nthr ** bigstar 0 nthr (shared_pre nthr Seq.Base.empty Seq.Base.empty 0 ar)
+  (nblk : sz { 0 < reveal nblk /\ reveal nblk <= max_blocks })
+  (nthr : sz { 0 < nthr /\ nthr <= max_threads })
+  (smem_sz : sz { smem_sz == SZ.(2sz *^ nthr) })
+  (ar: gpu_array u64 smem_sz)
+  (bid: sz { 0 <= bid /\ SZ.v bid < SZ.v nblk })
+  requires block_setup nthr ** (exists* v. gpu_pts_to_array #u64 #smem_sz ar #1.0R v)
+  ensures block_setup nthr ** bigstar 0 nthr (shared_pre nthr Seq.empty Seq.empty 0 ar)
 {
-  with v. assert (gpu_pts_to_array #U64.t #smem_sz ar #1.0R v);
+  with v. assert (gpu_pts_to_array #u64 #smem_sz ar #1.0R v);
   unfold gpu_pts_to_array ar v;
   gpu_slice_slice_1_underspec #1 ar #1.0R 0 smem_sz nthr;
   drop_   (bigstar #1 0 (SZ.v nthr - 0) (fun x -> gpu_pts_to_array1 ar (x + 0)));
@@ -77,16 +74,16 @@ fn block_setup_ghost
 
   bigstar_zip #1 #2 #1 0 nthr _ _;
 
-  mk_mbarrier nthr (barrier_mm nthr Seq.Base.empty Seq.Base.empty ar);
+  mk_mbarrier nthr (barrier_mm nthr Seq.empty Seq.empty ar);
   bigstar_zip #1 #0 #0 0 nthr _ _;
 
   // FOLD:
-  drop_   (bigstar #0 0 nthr (fun x -> gpu_pts_to_array1 ar x ** gpu_pts_to_array1 ar (x + nthr) ** mbarrier_tok nthr (barrier_mm nthr Seq.Base.empty Seq.Base.empty ar) 0 x));
-  assume_ (bigstar #0 0 nthr (fun x -> shared_pre nthr Seq.Base.empty Seq.Base.empty 0 ar x));
+  drop_   (bigstar #0 0 nthr (fun x -> gpu_pts_to_array1 ar x ** gpu_pts_to_array1 ar (x + nthr) ** mbarrier_tok nthr (barrier_mm nthr Seq.empty Seq.empty ar) 0 x));
+  assume_ (bigstar #0 0 nthr (fun x -> shared_pre nthr Seq.empty Seq.empty 0 ar x));
 
   bigstar_uneta();
   gpu_slice_empty_elim ar smem_sz;
 }
 
-let shared_post (nthr : SZ.t { 0 < nthr /\ nthr <= max_threads }) (ar: gpu_array U64.t SZ.(2sz *^ nthr)) (i: nat { 0 <= i /\ i < nthr }): slprop =
-  exists* it. shared_pre nthr Seq.Base.empty Seq.Base.empty it ar i
+let shared_post (nthr : sz { 0 < nthr /\ nthr <= max_threads }) (ar: gpu_array u64 SZ.(2sz *^ nthr)) (i: nat { 0 <= i /\ i < nthr }): slprop =
+  exists* it. shared_pre nthr Seq.empty Seq.empty it ar i
