src/examples/matmul/GPU.MatMul.Impure.fsti
@@ -9,7 +9,7 @@ open GPU
 module U64 = FStar.UInt64
 module SZ = FStar.SizeT
 
-let gpu_pts_to_matrix #a (rows columns: nat) (ga : gpu_array a (rows * columns)) (shared: erased nat{shared > 0}) (s: erased (Seq.Base.seq a)): slprop =
+let gpu_pts_to_matrix #a (rows columns: nat) (ga : gpu_array a (rows * columns)) (shared: erased nat{shared > 0}) (s: erased (seq a)): slprop =
   gpu_pts_to_array ga #(1.0R /. Real.of_int shared) s
 
 ghost
@@ -19,7 +19,7 @@ fn gpu_matrix_share_underspec
   (rows columns: nat)
   (ga : gpu_array a (rows * columns))
   (shared: erased nat{shared > 0})
-  (s: erased (Seq.Base.seq a) { Seq.length s == rows * columns })
+  (s: erased (seq a) { Seq.length s == rows * columns })
   requires gpu_pts_to_matrix #a rows columns ga 1 s
   ensures bigstar #uid 0 shared (fun _ -> gpu_pts_to_matrix #a rows columns ga shared s)
 
@@ -30,7 +30,7 @@ fn gpu_matrix_unshare_underspec
   (rows columns: nat)
   (ga : gpu_array a (rows * columns))
   (shared: erased nat{shared > 0})
-  (s: erased (Seq.Base.seq a) { Seq.length s == rows * columns })
+  (s: erased (seq a) { Seq.length s == rows * columns })
   requires bigstar #uid 0 shared (fun _ -> gpu_pts_to_matrix #a rows columns ga shared s)
   ensures  gpu_pts_to_matrix #a rows columns ga 1 s
 
@@ -41,16 +41,16 @@ fn gpu_matrix_unshare_underspec
 inline_for_extraction noextract
 fn gpu_matrix_read
   (#a:Type0)
-  (#rows #columns: SZ.t)
+  (#rows #columns: sz)
   (ga : gpu_array a (rows * columns))
   (#shared: erased nat{shared > 0})
-  (#s: erased (Seq.Base.seq a) { Seq.length s == rows * columns })
-  (row: SZ.t{SZ.v row < rows})
-  (col: SZ.t{SZ.v col < columns})
+  (#s: erased (seq a) { Seq.length s == rows * columns })
+  (row: sz{SZ.v row < rows})
+  (col: sz{SZ.v col < columns})
   requires gpu ** gpu_pts_to_matrix rows columns ga shared s
   returns v: a
   // TODO: is the assert here opaque?
-  ensures gpu ** gpu_pts_to_matrix rows columns ga shared s ** pure (assert ((SZ.v row + 1) * columns <= rows * columns); v == Seq.Base.index s (row * columns + SZ.v col))
+  ensures gpu ** gpu_pts_to_matrix rows columns ga shared s ** pure (assert ((SZ.v row + 1) * columns <= rows * columns); v == Seq.index s (row * columns + SZ.v col))
 {
   open FStar.SizeT;
   assume_ (pure (forall (x:nat). SizeT.fits x)); // CHEATING overflow
@@ -71,16 +71,16 @@ fn gpu_matrix_read
 [@@CPrologue "__device__"]
 inline_for_extraction noextract
 fn gpu_matrix_read_u64
-  (#rows #columns: SZ.t)
-  (ga : gpu_array U64.t (rows * columns))
+  (#rows #columns: sz)
+  (ga : gpu_array u64 (rows * columns))
   (#shared: erased nat{shared > 0})
-  (#s: erased (Seq.Base.seq U64.t) { Seq.length s == rows * columns })
-  (row: SZ.t{SZ.v row < rows})
-  (col: SZ.t{SZ.v col < columns})
+  (#s: erased (seq u64) { Seq.length s == rows * columns })
+  (row: sz{SZ.v row < rows})
+  (col: sz{SZ.v col < columns})
   requires gpu ** gpu_pts_to_matrix rows columns ga shared s
-  returns v: U64.t
+  returns v: u64
   // TODO: is the assert here opaque?
-  ensures gpu ** gpu_pts_to_matrix rows columns ga shared s ** pure (assert ((SZ.v row + 1) * columns <= rows * columns); v == Seq.Base.index s (row * columns + SZ.v col))
+  ensures gpu ** gpu_pts_to_matrix rows columns ga shared s ** pure (assert ((SZ.v row + 1) * columns <= rows * columns); v == Seq.index s (row * columns + SZ.v col))
 {
   open FStar.SizeT;
   assume_ (pure (forall (x:nat). SizeT.fits x)); // CHEATING overflow
@@ -89,7 +89,7 @@ fn gpu_matrix_read_u64
   // TODO: strange that commenting this out causes an error
   assert (pure ((row + 1) * columns <= rows * columns));
   let idx = row *^ columns +^ col;
-  let v = gpu_array_read #U64.t #(rows * columns) #0 #(rows * columns) ga #(Real.one /. Real.of_int shared) idx #s;
+  let v = gpu_array_read #u64 #(rows * columns) #0 #(rows * columns) ga #(Real.one /. Real.of_int shared) idx #s;
   fold gpu_pts_to_array ga #(Real.one /. Real.of_int shared) s;
   fold gpu_pts_to_matrix rows columns ga shared s;
   v
